Dataflow/Clocking/Properties.v
@@ -1,0 +1,86 @@
+Require Import Rustre.Common.
+Require Import Dataflow.Syntax.
+Require Import Dataflow.Clocking.
+Require Import Dataflow.Clocking.Parents.
+
+Require Import Dataflow.IsFree.
+Require Import Dataflow.IsDefined.
+
+Lemma Is_free_in_clock_self_or_parent:
+  forall x ck,
+    Is_free_in_clock x ck
+    -> exists ck' b, ck = Con ck' x b \/ clock_parent (Con ck' x b) ck.
+Proof.
+  Hint Constructors clock_parent.
+  induction ck as [|? IH]; [now inversion 1|].
+  intro Hfree.
+  inversion Hfree as [|? ? ? ? Hfree']; clear Hfree; subst.
+  - exists ck, b; now auto.
+  - specialize (IH Hfree'); clear Hfree'.
+    destruct IH as [ck' [b' Hcp]].
+    exists ck', b'; right.
+    destruct Hcp as [Hcp|Hcp]; [rewrite Hcp| inversion Hcp]; now auto.
+Qed.
+
+Theorem Well_clocked_eq_not_Is_free_in_clock:
+  forall C eq x ck,
+    Well_clocked_env C
+    -> Well_clocked_eq C eq
+    -> Is_defined_in_eq x eq
+    -> Has_clock_eq ck eq
+    -> ~Is_free_in_clock x ck.
+Proof.
+  intros C eq x ck Hwc Hwce Hdef Hhasck Hfree.
+  inversion Hwce as [x' ck' e Hcv Hexp Heq
+                    |x' ck' f e Hcv Hexp Heq
+                    |x' ck' v' e Hcv Hexp];
+    subst; inversion Hdef; inversion Hhasck; clear Hdef Hhasck; subst;
+    pose proof (Well_clocked_env_var _ _ _ Hwc Hcv) as Hclock;
+    apply Is_free_in_clock_self_or_parent in Hfree;
+    destruct Hfree as [ck [b [Hck|Hck]]];
+    (rewrite Hck in *;
+      apply clk_clock_sub with (1:=Hwc) in Hclock;
+      apply clk_var_det with (1:=Hcv) in Hclock;
+      apply clock_no_loops with (1:=Hclock))
+    ||
+    (apply clk_clock_parent with (1:=Hwc) (2:=Hck) in Hclock;
+      apply clk_clock_sub with (1:=Hwc) in Hclock;
+      apply clk_var_det with (1:=Hcv) in Hclock;
+      apply clock_parent_parent' in Hck;
+      rewrite <-Hclock in Hck;
+      apply clock_parent_not_refl with (1:=Hck)).
+Qed.
+
+Corollary Well_clocked_EqDef_not_Is_free_in_clock:
+  forall C x ce ck,
+    Well_clocked_env C
+    -> Well_clocked_eq C (EqDef x (CAexp ck ce))
+    -> ~Is_free_in_clock x ck.
+Proof.
+  intros C x ce ck Hwc Hwce.
+  apply Well_clocked_eq_not_Is_free_in_clock with (1:=Hwc) (2:=Hwce);
+    now constructor.
+Qed.
+
+Corollary Well_clocked_EqApp_not_Is_free_in_clock:
+  forall C x f le ck,
+    Well_clocked_env C
+    -> Well_clocked_eq C (EqApp x f (LAexp ck le))
+    -> ~Is_free_in_clock x ck.
+Proof.
+  intros C x f le ck Hwc Hwce.
+  apply Well_clocked_eq_not_Is_free_in_clock with (1:=Hwc) (2:=Hwce);
+    now constructor.
+Qed.
+
+Corollary Well_clocked_EqFby_not_Is_free_in_clock:
+  forall C x v0 le ck,
+    Well_clocked_env C
+    -> Well_clocked_eq C (EqFby x v0 (LAexp ck le))
+    -> ~Is_free_in_clock x ck.
+Proof.
+  intros C x v0 le ck Hwc Hwce.
+  apply Well_clocked_eq_not_Is_free_in_clock with (1:=Hwc) (2:=Hwce);
+    now constructor.
+Qed.
+
